Abstract proofs about hashtables.

mailbox/verif_hashtable1.v
@@ -28,16 +28,27 @@ Definition integer_hash_spec :=
   PRE [ _i OF tint ]
    PROP () LOCAL (temp _i (vint i)) SEP ()
   POST [ tint ]
-   EX i' : Z, PROP () LOCAL (temp ret_temp (vint i')) SEP ().
+   PROP () LOCAL (temp ret_temp (vint (i * 654435761))) SEP ().
+(* One might think it should just return an unknown number, but in fact it needs to follow a known hash
+   function at the logic level to be useful. *)
 
 Definition tentry := Tstruct _entry noattr.
 
 Definition entry_hists entries hists := fold_right sepcon emp (map (fun i =>
   let '(hp, e) := (Znth i hists ([], []), Znth i entries Vundef) in
     ghost_hist (fst hp) (field_address tentry [StructField _key] e) *
-    ghost_hist (snd hp) (field_address tentry [StructField _value] e)) (upto 20)).
+    ghost_hist (snd hp) (field_address tentry [StructField _value] e)) (upto 32)).
 
-(* In this case, let map be an association list. *)
+(* up *)
+Lemma Znth_cons : forall {A} (d : A) i x l, Znth i (x :: l) d = if eq_dec i 0 then x else Znth (i - 1) l d.
+Proof.
+  intros.
+  destruct (eq_dec i 0); [subst; apply Znth_0_cons|].
+  destruct (zlt i 0); [rewrite !Znth_underflow; auto; omega|].
+  apply Znth_pos_cons; omega.
+Qed.
+
+(* Maps are represented as partial association lists, with entries with key 0 considered to be empty. *)
 Fixpoint index_of (m : list (Z * Z)) (k : Z) :=
   match m with
   | [] => None
@@ -46,24 +57,277 @@ Fixpoint index_of (m : list (Z * Z)) (k : Z) :=
   end.
 
 Lemma index_of_spec : forall k m, match index_of m k with
-  | Some i => 0 <= i < Zlength m /\ fst (Znth i m (0, 0)) = k
+  | Some i => 0 <= i < Zlength m /\ fst (Znth i m (0, 0)) = k /\ Forall (fun x => fst x <> k) (sublist 0 i m)
   | None => ~In k (map fst m) end.
 Proof.
   induction m; simpl; auto; intros.
   destruct a.
   rewrite Zlength_cons.
   pose proof (Zlength_nonneg m).
-  destruct (eq_dec z k); [split; auto; omega|].
+  destruct (eq_dec z k).
+  { split; [omega|].
+    rewrite sublist_nil; auto. }
   destruct (index_of m k); simpl.
-  - destruct IHm; unfold Z.succ; rewrite Znth_pos_cons, Z.add_simpl_r; [split|]; auto; omega.
+  - destruct IHm as (? & ? & ?); unfold Z.succ.
+    rewrite Znth_cons, Z.add_simpl_r.
+    if_tac; [omega|].
+    split; [omega|].
+    split; auto.
+    rewrite sublist_0_cons, Z.add_simpl_r by omega; constructor; auto.
   - tauto.
 Qed.
 
-Definition set m k v :=
-  match index_of m k with
-  | Some i => upd_Znth i m (k, v)
-  | None => m ++ [(k, v)]
+(* Abstract properties of hashtables (of length 32) *)
+Definition hash i := (i * 654435761) mod 32.
+
+Definition well_chained (m : list (Z * Z)) := forall k i, index_of (rotate m (hash k) (Zlength m)) k = Some i ->
+  Forall (fun x => fst x <> 0) (sublist 0 i (rotate m (hash k) (Zlength m))).
+
+Definition wf_map (m : list (Z * Z)) := NoDup (map fst m).
+
+Definition indices i j := (map (fun x => (i + x) mod 32) (upto (Z.to_nat ((j - i) mod 32)))).
+
+Fixpoint index_of' (m : list (Z * Z)) k :=
+  match m with
+  | [] => None
+  | (k1, v1) :: rest => if eq_dec k1 0 then None else
+                        if eq_dec k1 k then Some 0
+                        else option_map Z.succ (index_of' rest k)
   end.
+
+Lemma index_of'_spec : forall k m, match index_of' m k with
+  | Some i => k <> 0 /\ 0 <= i < Zlength m /\ fst (Znth i m (0, 0)) = k /\
+              Forall (fun x => fst x <> 0 /\ fst x <> k) (sublist 0 i m)
+  | None => ~In k (map fst m) \/ exists i, 0 <= i < Zlength m /\ fst (Znth i m (0, 0)) = 0 /\
+            Forall (fun x => fst x <> 0 /\ fst x <> k) (sublist 0 i m) end.
+Proof.
+  induction m; simpl; auto; intros.
+  destruct a.
+  rewrite Zlength_cons.
+  pose proof (Zlength_nonneg m).
+  destruct (eq_dec z 0).
+  { subst; right.
+    exists 0; split; [omega|].
+    rewrite sublist_nil, Znth_cons; split; auto. }
+  destruct (eq_dec z k).
+  { subst; split; auto.
+    split; [omega|].
+    rewrite sublist_nil, Znth_cons; split; auto. }
+  destruct (index_of' m k); simpl.
+  - destruct IHm as (? & ? & ? & ?); unfold Z.succ; rewrite Znth_cons, Z.add_simpl_r.
+    split; auto.
+    if_tac; [omega|].
+    split; [omega|].
+    split; auto.
+    rewrite sublist_0_cons, Z.add_simpl_r by omega; constructor; auto.
+  - destruct IHm as [? | (i & ? & ? & ?)]; [tauto|].
+    right; exists (i + 1).
+    split; [omega|].
+    rewrite Znth_cons, sublist_0_cons, !Z.add_simpl_r by omega; if_tac; auto; omega.
+Qed.
+
+Definition lookup (m : list (Z * Z)) (k : Z) :=
+  option_map (fun i => (i - hash k) mod 32) (index_of' (rotate m (hash k) 32) k).
+
+(* up *)
+Lemma NoDup_Znth_inj : forall {A} (d : A) l i j (HNoDup : NoDup l)
+  (Hi : 0 <= i < Zlength l) (Hj : 0 <= j < Zlength l) (Heq : Znth i l d = Znth j l d),
+  i = j.
+Proof.
+  induction l; intros.
+  { rewrite Zlength_nil in *; omega. }
+  inv HNoDup.
+  rewrite Zlength_cons in *.
+  rewrite !Znth_cons in Heq.
+  destruct (eq_dec i 0), (eq_dec j 0); subst; auto.
+  - contradiction H1; apply Znth_In; omega.
+  - contradiction H1; apply Znth_In; omega.
+  - exploit (IHl (i - 1) (j - 1)); auto; omega.
+Qed.
+
+(* up *)
+Lemma Znth_rotate : forall {A} (d : A) i l n, 0 <= n <= Zlength l -> 0 <= i < Zlength l ->
+  Znth i (rotate l n (Zlength l)) d = Znth ((i - n) mod Zlength l) l d.
+Proof.
+  intros; unfold rotate.
+  destruct (zlt i n).
+  - rewrite app_Znth1 by (rewrite Zlength_sublist; omega).
+    rewrite Znth_sublist by omega.
+    rewrite <- Z_mod_plus with (b := 1), Zmod_small by omega.
+    f_equal; omega.
+  - rewrite app_Znth2; (rewrite Zlength_sublist; try omega).
+    rewrite Znth_sublist by omega.
+    rewrite Zmod_small by omega.
+    f_equal; omega.
+Qed.
+
+Lemma hash_range : forall i, 0 <= hash i < 32.
+Proof.
+  intro; apply Z_mod_lt; computable.
+Qed.
+
+Lemma rotate_In : forall {A} (x : A) n m l, 0 <= m - n <= Zlength l -> In x (rotate l n m) <-> In x l.
+Proof.
+  unfold rotate; intros.
+  replace l with (sublist 0 (m - n) l ++ sublist (m - n) (Zlength l) l) at 4
+    by (rewrite sublist_rejoin, sublist_same; auto; omega).
+  rewrite !in_app; tauto.
+Qed.
+
+Lemma index_of_app : forall k m1 m2, index_of (m1 ++ m2) k =
+  match index_of m1 k with Some i => Some i | None => option_map (Z.add (Zlength m1)) (index_of m2 k) end.
+Proof.
+  induction m1; simpl; intros.
+  - destruct (index_of m2 k); auto.
+  - destruct a.
+    destruct (eq_dec z k); auto.
+    rewrite IHm1; destruct (index_of m1 k); auto; simpl.
+    destruct (index_of m2 k); auto; simpl.
+    rewrite Zlength_cons; f_equal; omega.
+Qed.
+
+Lemma index_of_out : forall k m, Forall (fun x => fst x <> k) m -> index_of m k = None.
+Proof.
+  intros.
+  pose proof (index_of_spec k m) as Hk.
+  destruct (index_of m k); auto.
+  destruct Hk; eapply Forall_Znth in H; eauto.
+  subst; contradiction H; eauto.
+Qed.
+
+Lemma index_of_sublist : forall m a b i k (HNoDup : NoDup (map fst m))
+  (Hi : index_of (sublist a b m) k = Some i) (Ha : 0 <= a) (Hb : b <= Zlength m),
+  index_of m k = Some (i + a).
+Proof.
+  intros.
+  destruct (Z_le_dec b a); [rewrite sublist_nil_gen in Hi by auto; discriminate|].
+  assert (m = sublist 0 a m ++ sublist a b m ++ sublist b (Zlength m) m) as Hm.
+  { rewrite !sublist_rejoin, sublist_same; auto; omega. }
+  rewrite Hm, index_of_app, index_of_out, index_of_app, Hi; simpl.
+  rewrite Zlength_sublist by omega.
+  f_equal; omega.
+  { rewrite Hm, !map_app in HNoDup; apply NoDup_app in HNoDup.
+    destruct HNoDup as (_ & _ & HNoDup).
+    rewrite Forall_forall; intros ???.
+    exploit (HNoDup k); try contradiction.
+    * rewrite in_map_iff; eauto.
+    * rewrite in_app; left.
+      pose proof (index_of_spec k (sublist a b m)) as Hspec; rewrite Hi in Hspec.
+      destruct Hspec as (? & ? & ?).
+      rewrite in_map_iff; do 2 eexists; eauto.
+      apply Znth_In; auto. }
+Qed.
+
+Lemma index_of_rotate : forall m n k, 0 <= n <= Zlength m -> NoDup (map fst m) ->
+  index_of (rotate m n (Zlength m)) k = option_map (fun i => (i + n) mod Zlength m) (index_of m k).
+Proof.
+  intros.
+  destruct (eq_dec (Zlength m) 0).
+  { apply Zlength_nil_inv in e; subst.
+    unfold rotate; rewrite !sublist_of_nil; auto. }
+  unfold rotate; rewrite !index_of_app.
+  destruct (index_of (sublist (Zlength m - n) (Zlength m) m) k) eqn: Hk2.
+  - pose proof (index_of_spec k (sublist (Zlength m - n) (Zlength m) m)) as Hspec.
+    rewrite Hk2 in Hspec; destruct Hspec as (Hrange & ?).
+    apply index_of_sublist in Hk2; auto; try omega.
+    rewrite Hk2; simpl.
+    rewrite Zlength_sublist in Hrange by omega.
+    replace (z + _ + _) with (z + Zlength m) by omega.
+    rewrite Z.add_mod, Z_mod_same_full, Z.add_0_r, Zmod_mod by auto.
+    rewrite Zmod_small; auto; omega.
+  - replace (index_of m k) with
+      (index_of (sublist 0 (Zlength m - n) m ++ sublist (Zlength m - n) (Zlength m) m) k)
+      by (rewrite sublist_rejoin, sublist_same; auto; omega).
+    rewrite index_of_app, Hk2.
+    pose proof (index_of_spec k (sublist 0 (Zlength m - n) m)) as Hspec.
+    destruct (index_of (sublist 0 (Zlength m - n) m) k); auto; simpl.
+    rewrite Zlength_sublist in Hspec by omega.
+    rewrite Zlength_sublist, Zmod_small by omega.
+    f_equal; omega.
+Qed.
+
+Lemma Forall_sublist_first : forall {A} (P : A -> Prop) i j l d
+  (Hrangei : 0 <= i <= Zlength l) (Hi : Forall P (sublist 0 i l)) (Hi' : ~P (Znth i l d))
+  (Hrangej : 0 <= j <= Zlength l) (Hj : Forall P (sublist 0 j l)) (Hj' : ~P (Znth j l d)),
+  i = j.
+Proof.
+  intros.
+  destruct (zlt i j); [|destruct (zlt j i); [|omega]].
+  - eapply Forall_Znth with (i0 := i) in Hj; [|rewrite Zlength_sublist; omega].
+    rewrite Znth_sublist, Z.add_0_r in Hj by omega.
+    contradiction Hi'; eauto.
+  - eapply Forall_Znth with (i0 := j) in Hi; [|rewrite Zlength_sublist; omega].
+    rewrite Znth_sublist, Z.add_0_r in Hi by omega.
+    contradiction Hj'; eauto.
+Qed.
+
+Lemma index_of'_succeeds : forall k m i (Hi : 0 <= i < Zlength m)
+  (Hnz : Forall (fun x => fst x <> 0 /\ fst x <> k) (sublist 0 i m))
+  (Hk : fst (Znth i m (0, 0)) = k) (Hk' : k <> 0), index_of' m k = Some i.
+Proof.
+  intros.
+  pose proof (index_of'_spec k m).
+  destruct (index_of' m k).
+  - destruct H as (? & ? & Hz & Hnz').
+    f_equal; eapply Forall_sublist_first; eauto; simpl; try omega.
+    + rewrite Hz; tauto.
+    + rewrite Hk; tauto.
+  - destruct H as [? | (z & ? & Hz & ?)].
+    + contradiction H.
+      rewrite in_map_iff; do 2 eexists; eauto.
+      apply Znth_In; omega.
+    + assert (z = i); [|subst; contradiction Hk'].
+      eapply Forall_sublist_first; eauto; simpl; try omega.
+      * rewrite Hz; tauto.
+      * rewrite Hk; tauto.
+Qed.
+
+Lemma lookup_spec : forall m k (Hwf : wf_map m) (Hchain : well_chained m) (Hlen : Zlength m = 32)
+  (Hnz : k <> 0), lookup m k = index_of m k.
+Proof.
+  intros.
+  destruct (eq_dec (Zlength m) 0).
+  { apply Zlength_nil_inv in e; subst.
+    unfold lookup, rotate; rewrite !sublist_of_nil; auto. }
+  specialize (Hchain k).
+  pose proof (hash_range k).
+  assert (0 <= hash k <= Zlength m) by omega.
+  rewrite index_of_rotate in Hchain by auto.
+  unfold lookup.
+  pose proof (index_of_spec k m) as Hspec; destruct (index_of m k) eqn: Hk.
+  - specialize (Hchain _ eq_refl).
+    destruct Hspec as (? & Hz & ?).
+    assert (0 <= (z + hash k) mod Zlength m < Zlength m) by (apply Z_mod_lt; omega).
+    assert (((z + hash k) mod Zlength m - hash k) mod Zlength m = z) as Hmod.
+    { rewrite Zminus_mod_idemp_l, Z.add_simpl_r, Zmod_small; auto. }
+    assert (fst (Znth ((z + hash k) mod Zlength m) (rotate m (hash k) 32) (0, 0)) = k).
+    { rewrite <- Hlen, Znth_rotate, Hmod; auto. }
+    erewrite index_of'_succeeds; eauto; simpl.
+    rewrite <- Hlen, Hmod; auto.
+    + rewrite Zlength_rotate; auto; omega.
+    + rewrite Forall_forall; intros ? Hin.
+      split; [rewrite Forall_forall in Hchain; apply Hchain; rewrite !Hlen in *; auto|].
+      intro Heq; apply In_Znth with (d := (0, 0)) in Hin.
+      destruct Hin as (i & Hi & ?); subst x.
+      rewrite Zlength_sublist in Hi; try omega.
+      rewrite Znth_sublist, <- Hlen, Znth_rotate, Z.add_0_r in Heq by omega.
+      eapply NoDup_Znth_inj with (i0 := z)(j := (i - hash k) mod (Zlength m)) in Hwf.
+      subst z.
+      rewrite Zplus_mod_idemp_l, Z.sub_simpl_r, Z.sub_0_r, Zmod_small in Hi; try omega.
+      * destruct Hi; split; auto.
+        etransitivity; eauto.
+        apply Z_mod_lt; omega.
+      * rewrite Zlength_map; auto.
+      * rewrite Zlength_map; apply Z_mod_lt; omega.
+      * rewrite !Znth_map'; subst k; eauto.
+      * rewrite Zlength_rotate; omega.
+  - pose proof (index_of'_spec k (rotate m (hash k) 32)) as Hspec'; destruct (index_of' _ _); auto.
+    destruct Hspec' as (? & Hrange & Hz & ?); contradiction Hspec.
+    rewrite Zlength_rotate in Hrange by omega.
+    rewrite <- Hlen, Znth_rotate in Hz by auto.
+    rewrite in_map_iff; do 2 eexists; eauto.
+    apply Znth_In, Z_mod_lt; omega.
+Qed.
 
 Definition get m k := option_map (fun i => snd (Znth i m (0, 0))) (index_of m k).
 
@@ -172,8 +436,6 @@ Proof.
     rewrite app_Znth1 by omega; apply H; auto; omega.
 Qed.
 
-Definition wf_map (m : list (Z * Z)) := Forall (fun i => repable_signed i /\ i <> 0) (map fst m).
-
 Definition int_op e :=
   match e with
   | Load v | Store v => tc_val tint v
@@ -192,10 +454,9 @@ Definition atomic_entry sh p := !!(field_compatible tentry [] p) && EX lkey : va
   field_at sh tentry [StructField _lvalue] lval p *
   atomic_loc sh lval (field_address tentry [StructField _value] p) (vint 0) Tsh v_R.
 
-Definition wf_hists h l := Forall (fun x => (ordered_hist (fst x) /\ Forall int_op (map snd (fst x))) /\
-  (ordered_hist (snd x) /\ Forall int_op (map snd (snd x)))) h /\ 0 <= l <= Zlength h /\
-    Forall (fun x => value_of_hist (fst x) <> vint 0) (sublist 0 l h) /\
-    Forall (fun x => value_of_hist (fst x) = vint 0) (sublist l (Zlength h) h).
+(* Entries are no longer consecutive. *)
+Definition wf_hists h := Forall (fun x => (ordered_hist (fst x) /\ Forall int_op (map snd (fst x))) /\
+  (ordered_hist (snd x) /\ Forall int_op (map snd (snd x)))) h.
 
 Definition make_int v := match v with Vint i => Int.signed i | _ => 0 end.
 
@@ -205,31 +466,14 @@ Proof.
   rewrite Int.repr_signed; auto.
 Qed.
 
-Fixpoint make_map h :=
-  match h with
-  | [] => []
-  | (hk, hv) :: rest => let k := make_int (value_of_hist hk) in
-      if eq_dec k 0 then [] else (k, make_int (value_of_hist hv)) :: make_map rest
-  end.
-
-Lemma Forall_set : forall P m k v, Forall P m -> P (k, v) -> Forall P (set m k v).
+Lemma make_int_repable : forall v, repable_signed (make_int v).
 Proof.
-  intros; unfold set.
-  destruct (index_of m k).
-  - apply Forall_upd_Znth; auto.
-  - rewrite Forall_app; split; auto.
-Qed.
-
-Lemma wf_make_map : forall h, wf_map (make_map h).
-Proof.
-  unfold wf_map; induction h; simpl; auto.
-  destruct a.
-  if_tac; simpl; auto.
-  constructor; auto.
-  split; auto.
-  destruct (value_of_hist _); simpl; try (split; computable).
+  destruct v; simpl; try (split; computable).
   apply Int.signed_range.
 Qed.
+
+Definition make_map h :=
+  map (fun hs => (make_int (value_of_hist (fst hs)), make_int (value_of_hist (snd hs)))) h.
 
 Lemma make_map_eq : forall h h', Forall2 (fun a b => value_of_hist (fst a) = value_of_hist (fst b) /\
   value_of_hist (snd a) = value_of_hist (snd b)) h h' -> make_map h = make_map h'.
@@ -253,83 +497,13 @@ Proof.
   simpl; intros; apply int_op_value; auto.
 Qed.
 
-Lemma make_map_app : forall h1 h2 (Hnz : Forall (fun x => value_of_hist (fst x) <> vint 0) h1)
-  (Hint : Forall (fun x => Forall int_op (map snd (fst x))) h1),
-  make_map (h1 ++ h2) = make_map h1 ++ make_map h2.
-Proof.
-  induction 1; auto; simpl; intros.
-  inv Hint.
-  destruct x as (h, ?).
-  rewrite IHHnz; auto.
-  if_tac; auto.
-  exploit int_op_value_of_hist; eauto; simpl.
-  destruct (value_of_hist h) eqn: Hval; try contradiction; simpl in *.
-  contradiction H; rewrite Hval.
-  f_equal; apply signed_inj; auto.
-Qed.
-
-Lemma make_map_drop : forall h1 h2 (Hz : Forall (fun x => value_of_hist (fst x) = vint 0) h2),
-  make_map (h1 ++ h2) = make_map h1.
-Proof.
-  induction h1; simpl; intros.
-  - destruct h2; auto; simpl.
-    destruct p as (h, ?).
-    if_tac; auto.
-    inv Hz.
-    contradiction H; simpl in *.
-    replace (value_of_hist h) with (vint 0); auto.
-  - rewrite IHh1; auto.
-Qed.
-
-Lemma index_of_app : forall k m1 m2, index_of (m1 ++ m2) k =
-  match index_of m1 k with Some i => Some i | None => option_map (Z.add (Zlength m1)) (index_of m2 k) end.
-Proof.
-  induction m1; simpl; intros.
-  - destruct (index_of m2 k); auto.
-  - destruct a.
-    destruct (eq_dec z k); auto.
-    rewrite IHm1; destruct (index_of m1 k); auto; simpl.
-    destruct (index_of m2 k); auto; simpl.
-    rewrite Zlength_cons; f_equal; omega.
-Qed.
-
-Lemma index_of_out : forall k m, Forall (fun x => fst x <> k) m -> index_of m k = None.
-Proof.
-  intros.
-  pose proof (index_of_spec k m) as Hk.
-  destruct (index_of m k); auto.
-  destruct Hk; eapply Forall_Znth in H; eauto.
-  subst; contradiction H; eauto.
-Qed.
-
-Lemma make_map_length : forall h (Hnz : Forall (fun x => value_of_hist (fst x) <> vint 0) h)
-  (Hint : Forall (fun x => Forall int_op (map snd (fst x))) h),
-  Zlength (make_map h) = Zlength h.
-Proof.
-  induction h; auto; simpl; intros.
-  inv Hnz; inv Hint.
-  destruct a as (hk, ?); simpl in *.
-  exploit int_op_value_of_hist; eauto.
-  destruct (value_of_hist hk); try contradiction; simpl.
-  if_tac; [|rewrite !Zlength_cons, IHh; auto].
-  absurd (Vint i = vint 0); auto; f_equal; apply signed_inj; auto.
-Qed.
-
 Lemma make_map_no_key : forall h k (Hout : Forall (fun x => make_int (value_of_hist (fst x)) <> k) h),
   Forall (fun x => fst x <> k) (make_map h).
 Proof.
   induction h; simpl; auto; intros.
   destruct a.
   inv Hout.
-  if_tac; auto.
-Qed.
-
-Lemma make_map_nil : forall h, Forall (fun x => value_of_hist (fst x) = vint 0) h -> make_map h = [].
-Proof.
-  destruct h; auto; simpl.
-  destruct p.
-  intro H; inversion H as [|?? Heq]; subst.
-  simpl in *; rewrite Heq; auto.
+  constructor; auto.
 Qed.
 
 Definition failed_CAS k (a b : hist * hist) := exists t r, newer (fst a) t /\
@@ -338,8 +512,8 @@ Definition failed_CAS k (a b : hist * hist) := exists t r, newer (fst a) t /\
   r <> Int.zero /\ r <> Int.repr k /\ snd b = snd a /\
   (let v := value_of_hist (fst a) in v <> vint 0 -> v = Vint r).
 
-Definition set_item_trace (h : list (hist * hist)) k v i h' := 0 <= i < Zlength h /\
-  Forall2 (failed_CAS k) (sublist 0 i h) (sublist 0 i h') /\
+Definition set_item_trace (h : list (hist * hist)) k v i h' := Zlength h' = Zlength h /\
+  0 <= i < Zlength h /\
   (let '(hk, hv) := Znth i h ([], []) in exists t r tv, newer hk t /\ newer hv tv /\
      (fst (Znth i h' ([], [])) = hk ++ [(t, Load (vint k))] /\ r = vint k \/
       exists t1, (t < t1)%nat /\
@@ -347,49 +521,51 @@ Definition set_item_trace (h : list (hist * hist)) k v i h' := 0 <= i < Zlength 
         (r = vint 0 \/ r = vint k)) /\
      snd (Znth i h' ([], [])) = hv ++ [(tv, Store (vint v))] /\
      (let v := value_of_hist hk in v <> vint 0 -> v = r)) /\
-  sublist (i + 1) (Zlength h) h = sublist (i + 1) (Zlength h') h'.
+  forall j, (In j (indices (hash k) i) -> failed_CAS k (Znth j h ([], [])) (Znth j h' ([], []))) /\
+    (~In j (indices (hash k) i) -> j <> i -> Znth j h' ([], []) = Znth j h ([], [])).
 
+(* up *)
 Lemma app_cons_assoc : forall {A} l1 (x : A) l2, l1 ++ x :: l2 = (l1 ++ [x]) ++ l2.
 Proof.
   intros; rewrite <- app_assoc; auto.
 Qed.
 
-Lemma set_item_trace_map : forall h k v i h' l (Hwf : wf_hists h l) (Htrace : set_item_trace h k v i h')
+Definition map_incl (m m' : list (Z * Z)) := forall k v i, k <> 0 -> Znth i m (0, 0) = (k, v) ->
+  Znth i m' (0, 0) = (k, v).
+
+(* up *)
+Lemma Forall_forall_Znth : forall {A} (P : A -> Prop) l d,
+  Forall P l <-> forall i, 0 <= i < Zlength l -> P (Znth i l d).
+Proof.
+  split; intros; [apply Forall_Znth; auto|].
+  induction l; auto.
+  rewrite Zlength_cons in *.
+  constructor.
+  - specialize (H 0); rewrite Znth_0_cons in H; apply H.
+    pose proof (Zlength_nonneg l); omega.
+  - apply IHl; intros.
+    specialize (H (i + 1)).
+    rewrite Znth_pos_cons, Z.add_simpl_r in H by omega.
+    apply H; omega.
+Qed.
+
+Lemma set_item_trace_map : forall h k v i h' (Hwf : wf_hists h) (Hm : wf_map (make_map h))
+  (Htrace : set_item_trace h k v i h')
   (Hk : k <> 0) (Hrepk : repable_signed k) (Hrepv : repable_signed v),
-  wf_hists h' (Z.max (i + 1) l) /\ let m' := make_map (sublist 0 i h' ++ sublist i (Zlength h) h) in
-    wf_map (set m' k v) /\ incl (make_map h) m' /\ make_map h' = set m' k v.
+  wf_hists h' /\ let m' := make_map (upd_Znth i h' (Znth i h ([], []))) in
+    map_incl (make_map h) m' /\ make_map h' = upd_Znth i m' (k, v) /\ wf_map (make_map h').
 Proof.
   intros.
-  destruct Htrace as (Hbounds & Hfail & Hi & Hrest).
+  destruct Htrace as (Hlen & Hbounds & Hi & Hrest).
   destruct (Znth i h ([], [])) as (hk, hv) eqn: Hhi.
   destruct Hi as (t & r & tv & Ht & Htv & Hi1 & Hi2 & Hr0).
-  assert (Zlength h' = Zlength h) as Hlen.
-  { exploit (Znth_inbounds i h' ([], [])).
-    { destruct (Znth i h' ([], [])); intro X; inv X.
-      apply app_cons_not_nil in Hi2; auto. }
-    intro.
-    assert (Zlength (sublist (i + 1) (Zlength h) h) = Zlength (sublist (i + 1) (Zlength h') h')) as Heq
-      by (rewrite Hrest; auto).
-    rewrite !Zlength_sublist in Heq; omega. }
   assert (i <= Zlength h') by (rewrite Hlen; destruct Hbounds; apply Z.lt_le_incl; auto).
   assert (0 <= i + 1 <= Zlength h').
   { rewrite Hlen; destruct Hbounds; split; [|rewrite <- lt_le_1]; auto; omega. }
-  destruct Hwf as (Hwf & ? & Hl1 & Hl2).
   assert (vint k <> vint 0).
   { intro; contradiction Hk; apply repr_inj_signed; auto.
     { split; computable. }
     { congruence. }}
-  assert (Forall (fun x => value_of_hist (fst x) <> vint 0) (sublist 0 i h')).
-  { rewrite Forall_forall; intros (?, ?) Hin.
-    exploit (Forall2_In_r (failed_CAS k)); eauto.
-    intros ((?, ?) & ? & ? & r1 & ? & [? | (? & ? & ?)] & ? & ? & ? & ?); simpl in *; subst.
-    - unfold value_of_hist; rewrite last_snoc; simpl.
-      intro X; absurd (r1 = Int.zero); auto; inv X; auto.
-    - rewrite app_cons_assoc.
-      unfold value_of_hist; rewrite last_snoc; simpl.
-      destruct (eq_dec (Vint r1) (vint 0)); auto. }
-  assert (h' = sublist 0 i h' ++ Znth i h' ([], []) :: sublist (i + 1) (Zlength h') h') as Hh'.
-  { rewrite <- sublist_next, sublist_rejoin, sublist_same; auto; try omega; rewrite Hlen; auto. }
   assert (r = vint 0 \/ r = vint k) as Hr.
   { destruct Hi1 as [(? & ?) | (? & ? & ? & ?)]; auto. }
   assert ((if eq_dec r (vint 0) then vint k else r) = vint k) as Hif.
@@ -399,175 +575,61 @@ Proof.
   { destruct Hi1 as [(-> & ?) | (? & ? & -> & ?)].
     - unfold value_of_hist; rewrite last_snoc; auto.
     - rewrite app_cons_assoc; unfold value_of_hist; rewrite last_snoc; auto. }
-  assert (wf_hists h' (Z.max (i + 1) l)) as Hwf'; [|split; auto; split; [|split]].
-  - split.
-    + rewrite Hh'; clear Hh'; rewrite Forall_app; split; [|constructor].
-      * rewrite Forall_forall; intros (?, ?) Hin.
-        exploit (Forall2_In_r (failed_CAS k)); eauto.
-        intros ((?, ?) & Hin' & ? & ? & ? & Hcase & ? & ? & ? & ?); simpl in *; subst.
-        apply sublist_In in Hin'; rewrite Forall_forall in Hwf; destruct (Hwf _ Hin') as ((? & ?) & ?).
-        split; auto.
-        destruct Hcase as [? | (? & ? & ?)]; subst; rewrite map_app, Forall_app; repeat constructor; auto.
-        { apply ordered_snoc; auto. }
-        { rewrite app_cons_assoc; apply ordered_snoc; [apply ordered_snoc; auto|].
-          apply newer_snoc; auto. }
-      * eapply Forall_Znth with (i0 := i) in Hwf; auto.
-        rewrite Hhi in Hwf; destruct Hwf as ((? & ?) & ? & ?).
-        split; [|rewrite Hi2, map_app, Forall_app; repeat constructor; auto; apply ordered_snoc; auto].
-        destruct Hi1 as [(-> & _) | (? & ? & -> & _)]; rewrite map_app, Forall_app; repeat constructor;
-          auto; try (apply ordered_snoc; auto).
-        { rewrite app_cons_assoc; apply ordered_snoc; [apply ordered_snoc; auto|].
-          apply newer_snoc; auto. }
-        destruct Hr; subst; simpl; auto.
-      * rewrite <- Hrest; apply Forall_sublist; auto.
-    + assert (0 <= Z.max (i + 1) l <= Zlength h'); [|split; auto].
-      { destruct (Z.max_spec (i + 1) l) as [(? & ->) | (? & ->)]; auto; omega. }
-      split; [|apply Forall_suffix_max with (l1 := h); auto; omega].
-      rewrite Hh'; clear Hh'.
-      assert (Zlength h' <= i - 0 + Z.succ (Zlength h' - (i + 1))) by omega.
-      assert (0 <= Zlength h' - i) by omega.
-      destruct (Z.max_spec (i + 1) l) as [(? & ->) | (? & ->)].
-      * rewrite !sublist_app; rewrite ?Zlength_cons, ?Zlength_sublist; auto; try omega.
-        rewrite Z.min_l, Z.min_r, Z.max_r, Z.max_l by omega.
-        rewrite !Z.sub_0_r.
-        rewrite sublist_sublist, !Z.add_0_r by omega.
-        rewrite Forall_app; split; auto.
-        rewrite sublist_0_cons by omega.
-        constructor; [rewrite Hk'; auto|].
-        rewrite sublist_sublist by omega.
-        rewrite <- Z.sub_add_distr, Z.sub_simpl_r.
-        rewrite Z.add_0_l, sublist_parts2; try omega.
-        rewrite <- Hrest.
-        rewrite <- sublist_parts2 by omega.
-        rewrite sublist_parts1 by omega; apply Forall_sublist; auto.
-      * rewrite !sublist_app; rewrite ?Zlength_cons, ?Zlength_sublist; auto; try omega.
-        rewrite !Z.sub_0_r, Z.min_l, Z.min_r, Z.max_r, Z.max_l; auto; try omega.
-        rewrite Z.add_simpl_l.
-        rewrite sublist_same, sublist_len_1 with (d := ([], [])), Znth_0_cons;
-          rewrite ?Zlength_cons, ?Zlength_sublist; auto; try omega; simpl.
-        rewrite Forall_app; split; auto.
-        constructor; auto; rewrite Hk'; auto.
-  - unfold wf_map; rewrite Forall_map; apply Forall_set; auto.
-    rewrite <- Forall_map; apply wf_make_map.
-  - clear Hh'; match goal with H : 0 <= l <= _ |- _ => destruct H end.
-    assert (Forall2 (fun a b => value_of_hist (fst a) = value_of_hist (fst b) /\
-      value_of_hist (snd a) = value_of_hist (snd b)) (sublist 0 (Z.min i l) h) (sublist 0 (Z.min i l) h')) as Heq.
-    { rewrite Forall2_eq_upto with (d1 := ([] : hist, [] : hist))(d2 := ([] : hist, [] : hist)).
-      assert (0 <= Z.min i l <= Zlength h) as (? & ?).
-      { split; [rewrite Z.min_glb_iff | rewrite Z.min_le_iff]; auto; omega. }
-      split; [rewrite !Zlength_sublist; auto; omega|].
-      rewrite Forall_forall; intros ? Hin.
-      rewrite In_upto, Z2Nat.id in Hin by (apply Zlength_nonneg).
-      assert (value_of_hist (fst (Znth x (sublist 0 (Z.min i l) h) ([], []))) <> vint 0) as Hnz.
-      { apply Forall_Znth; auto.
-        rewrite <- sublist_prefix; apply Forall_sublist; auto. }
-      rewrite Zlength_sublist, Z.sub_0_r in Hin by (auto; omega).
-      assert (x < i).
-      { destruct Hin; eapply Z.lt_le_trans; eauto.
-        apply Z.le_min_l. }
-      exploit (Forall2_Znth _ _ _ ([], []) ([], []) Hfail x); auto.
-      { rewrite Zlength_sublist; omega. }
-      intros (? & r1 & ? & Heq1 & ? & ? & Heq2 & Hv).
-      rewrite !Znth_sublist, Z.add_0_r in Heq1, Heq2, Hv, Hnz; auto; try omega.
-      rewrite !Znth_sublist, Z.add_0_r in Heq2 by omega.
-      rewrite !Znth_sublist, Z.add_0_r by omega.
-      rewrite Heq2; split; auto.
-      destruct Heq1 as [-> | (? & ? & ->)].
-      + unfold value_of_hist at 2; rewrite last_snoc; auto.
-      + rewrite app_cons_assoc; unfold value_of_hist at 2; rewrite last_snoc; simpl.
-        destruct (eq_dec (Vint r1) (vint 0)); [absurd (r1 = Int.zero); auto; inv e|]; auto. }
-    replace h with (sublist 0 l h ++ sublist l (Zlength h) h) at 1
-      by (rewrite sublist_rejoin, sublist_same; auto; omega).
-    rewrite make_map_drop; auto.
-    assert (Forall (fun x => Forall int_op (map snd (fst x))) h').
-    { destruct Hwf'; eapply Forall_impl; [|eauto]; tauto. }
-    destruct (Z.min_spec i l) as [(? & Hmin) | (? & Hmin)]; rewrite Hmin in *; clear Hmin.
-    + assert (Forall (fun x : hist * hist => value_of_hist (fst x) <> vint 0) (sublist 0 i h')).
-      { eapply Forall_Forall2; try apply Heq.
-        { replace i with (Z.min i l) by (apply Z.min_l; omega).
-          rewrite <- sublist_prefix; apply Forall_sublist; auto. }
-        intros ??? (<- & _); auto. }
-      assert (Forall (fun x => Forall int_op (map snd (fst x))) (sublist 0 i h'))
-        by (apply Forall_sublist; auto).
-      rewrite make_map_app; auto.
-      rewrite sublist_split with (lo := i)(mid := l) by omega.
-      rewrite make_map_app, app_assoc.
-      apply incl_appl.
-      rewrite <- make_map_app; auto.
-      erewrite make_map_eq; [apply incl_refl|].
-      rewrite sublist_split with (mid := i) by omega.
-      apply Forall2_app; auto.
-      rewrite Forall2_eq_upto with (d1 := ([] : hist, [] : hist))(d2 := ([] : hist, [] : hist)).
-      split; auto; rewrite Forall_forall; intros; auto.
-      * rewrite sublist_parts1 by omega; apply Forall_sublist; auto.
-      * apply Forall_sublist; eapply Forall_impl, Hwf; tauto.
-    + rewrite sublist_split with (mid := l)(hi := i) by omega.
-      rewrite <- app_assoc, make_map_app.
-      apply incl_appl.
-      erewrite make_map_eq; [apply incl_refl | auto].
-      * eapply Forall_Forall2; try apply Heq; auto.
-        intros ??? (<- & _); auto.
-      * apply Forall_sublist; auto.
-  - unfold set.
-    destruct Hwf' as (? & ? & Hl1' & ?).
-    assert (Forall (fun x => Forall int_op (map snd (fst x))) (sublist 0 i h')).
-    { eapply Forall_sublist, Forall_impl; [|eauto]; tauto. }
-    rewrite Hh' at 1; clear Hh'.
-    rewrite make_map_app by auto.
-    assert (Forall (fun x => make_int (value_of_hist (fst x)) <> k) (sublist 0 i h')) as Hmiss.
-    { rewrite Forall_forall; intros (hk', hv') Hin.
-      exploit (Forall2_In_r _ (hk', hv') _ _ Hfail); auto.
-      intros (? & ? & ? & r1 & ? & Heqi & ? & ? & ? & ?); simpl in *; subst.
-      destruct Heqi as [-> | (? & ? & ->)].
-      + unfold value_of_hist; rewrite last_snoc; simpl.
-        intro; absurd (r1 = Int.repr k); auto; apply signed_inj; auto.
-        rewrite Int.signed_repr; auto.
-      + rewrite app_cons_assoc; unfold value_of_hist; rewrite last_snoc; simpl.
-        destruct (eq_dec (Vint r1) (vint 0)); simpl.
-        { absurd (r1 = Int.zero); auto; inv e; auto. }
-        intro; absurd (r1 = Int.repr k); subst; auto.
-        rewrite Int.repr_signed; auto. }
-    rewrite make_map_app at 1 by auto.
-    rewrite index_of_app, index_of_out, make_map_length by (auto; apply make_map_no_key; auto); simpl.
-    destruct (Znth i h' ([], [])) eqn: Hhi'; simpl in *.
-    rewrite Hk'; subst; simpl.
-    unfold value_of_hist; rewrite last_snoc; simpl.
-    rewrite !Int.signed_repr; auto.
-    destruct (eq_dec k 0); [contradiction Hk; auto|].
-    destruct (zlt i l).
-    + destruct (eq_dec (value_of_hist hk) (vint 0)).
-      { eapply Forall_Znth with (i0 := i) in Hl1; [|rewrite Zlength_sublist; omega].
-        rewrite Znth_sublist, Z.add_0_r, Hhi in Hl1 by omega; contradiction Hl1. }
-      assert (value_of_hist hk = vint k) as Hik.
-      { rewrite Hr0; auto.
-        rewrite Hr0 in n0; auto.
-        destruct Hr; [contradiction n0; auto | auto]. }
-      erewrite sublist_next with (i0 := i), Hhi by omega; simpl.
-      rewrite Hik; simpl.
+  assert (wf_hists h') as Hwf'; [|split; auto; split; [|split]].
+  - unfold wf_hists; rewrite Forall_forall_Znth; intros j ?.
+    apply (Forall_Znth _ _ j ([], [])) in Hwf; [destruct Hwf as ((? & ?) & ? & ?) | omega].
+    destruct (eq_dec j i); [|specialize (Hrest j); destruct (in_dec Z_eq_dec j (indices (hash k) i))].
+    + subst; rewrite Hhi in *.
+      split; [|rewrite Hi2, map_app, Forall_app; repeat constructor; auto; apply ordered_snoc; auto].
+      destruct Hi1 as [(-> & _) | (? & ? & -> & _)]; rewrite map_app, Forall_app; repeat constructor;
+        auto; try (apply ordered_snoc; auto).
+      * rewrite app_cons_assoc; apply ordered_snoc; [apply ordered_snoc; auto|].
+        apply newer_snoc; auto.
+      * destruct Hr; subst; simpl; auto.
+    + destruct Hrest as ((? & ? & ? & Hcase & ? & ? & -> & ?) & _); auto; simpl in *.
+      split; auto.
+      destruct Hcase as [-> | (? & ? & ->)]; rewrite map_app, Forall_app; repeat constructor; auto.
+      * apply ordered_snoc; auto.
+      * rewrite app_cons_assoc; apply ordered_snoc; [apply ordered_snoc; auto|].
+        apply newer_snoc; auto.
+    + destruct Hrest as (_ & ->); auto.
+  - intros k0 v0 j Hk0 Hj.
+    exploit (Znth_inbounds j (make_map h) (0, 0)).
+    { rewrite Hj; intro X; inv X; contradiction Hk0; auto. }
+    intro; unfold make_map in *; rewrite <- upd_Znth_map.
+    rewrite Zlength_map in *.
+    rewrite Znth_map with (d' := ([], [])) in Hj by auto; inv Hj.
+    destruct (eq_dec j i); [subst; rewrite upd_Znth_same, Hhi; auto | rewrite upd_Znth_diff];
+      rewrite ?Zlength_map in *; auto; try omega.
+    rewrite Znth_map with (d' := ([], [])) by omega.
+    specialize (Hrest j); destruct (in_dec Z_eq_dec j (indices (hash k) i));
+      [|destruct Hrest as (_ & ->); auto].
+    destruct Hrest as ((? & r1 & ? & Hcase & ? & ? & -> & Heq) & _); auto; simpl in *.
+    assert (value_of_hist (fst (Znth j h ([], []))) <> vint 0).
+    { intro X; rewrite X in Hk0; contradiction Hk0; auto. }
+    destruct Hcase as [-> | (? & ? & ->)].
+    + unfold value_of_hist at 1; rewrite last_snoc, Heq; auto.
+    + rewrite app_cons_assoc; unfold value_of_hist at 1; rewrite last_snoc, Heq; auto; simpl.
+      destruct (eq_dec (Vint r1) (vint 0)); auto.
+      absurd (r1 = Int.zero); auto; inv e; auto.
+  - assert (0 <= i < Zlength h') by (rewrite Hlen; auto).
+    unfold make_map; rewrite <- upd_Znth_map, upd_Znth_twice by (rewrite Zlength_map; auto).
+    apply list_Znth_eq' with (d := (0, 0)).
+    { rewrite upd_Znth_Zlength; auto.
+      rewrite Zlength_map; auto. }
+    rewrite Zlength_map; intros.
+    destruct (eq_dec j i); [subst; rewrite upd_Znth_same; auto | rewrite upd_Znth_diff];
+      rewrite ?Zlength_map; auto.
+    rewrite Znth_map with (d' := ([], [])) by omega.
+    unfold value_of_hist at 2; rewrite Hi2, last_snoc; simpl.
+    rewrite Int.signed_repr by auto.
+    destruct Hi1 as [(-> & ?) | (? & ? & -> & ?)].
+    + unfold value_of_hist; rewrite last_snoc; simpl.
       rewrite Int.signed_repr; auto.
-      destruct (eq_dec k 0); [contradiction Hk; auto | simpl].
-      rewrite eq_dec_refl; simpl.
-      rewrite make_map_app, Z.add_0_r by auto.
-      rewrite upd_Znth_app2; rewrite make_map_length; auto.
-      rewrite Zminus_diag, upd_Znth0; simpl.
-      rewrite Hik; simpl.
+    + unfold value_of_hist; rewrite app_cons_assoc, last_snoc; simpl.
+      rewrite Hif; simpl.
       rewrite Int.signed_repr; auto.
-      destruct (eq_dec k 0); [contradiction Hk; auto | simpl].
-      rewrite sublist_1_cons, Zlength_cons.
-      unfold Z.succ; rewrite Z.add_simpl_r.
-      rewrite sublist_same with (hi := Zlength (make_map _)), Hrest; auto.
-      { pose proof (Zlength_nonneg (make_map ((hk, hv) :: sublist (i + 1) (Zlength h) h))); omega. }
-    + erewrite sublist_next with (i0 := i) at 1 by omega; simpl.
-      exploit (Forall_Znth (fun x => value_of_hist (fst x) = vint 0) (sublist l (Zlength h) h) (i - l)); auto.
-      { rewrite Zlength_sublist; omega. }
-      rewrite Znth_sublist, Z.sub_simpl_r, Hhi by omega; simpl.
-      rewrite Hhi; intros ->; simpl.
-      rewrite make_map_nil with (h := sublist (i + 1) _ _).
-      rewrite make_map_drop; auto.
-      { replace i with (i - l + l) by (apply Z.sub_simpl_r).
-        rewrite <- sublist_suffix by omega; apply Forall_sublist; auto. }
-      { rewrite <- Hrest; replace (i + 1) with (i + 1 - l + l) by (apply Z.sub_simpl_r).
-        rewrite <- sublist_suffix by omega; apply Forall_sublist; auto. }
+  - repeat intro.
 Qed.
 
 (* What can a thread know?
@@ -575,19 +637,19 @@ Qed.
    It can even rely on the indices of known keys. *)
 Definition set_item_spec :=
  DECLARE _set_item
-  WITH key : Z, value : Z, p : val, sh : share, entries : list val, h : list (hist * hist), l : Z
+  WITH key : Z, value : Z, p : val, sh : share, entries : list val, h : list (hist * hist)
   PRE [ _key OF tint, _value OF tint ]
    PROP (repable_signed key; repable_signed value; readable_share sh; key <> 0; Forall isptr entries;
-         Zlength h = 20; wf_hists h l)
+         Zlength h = 32; wf_hists h)
    LOCAL (temp _key (vint key); temp _value (vint value); gvar _m_entries p)
-   SEP (data_at sh (tarray (tptr tentry) 20) entries p;
+   SEP (data_at sh (tarray (tptr tentry) 32) entries p;
         fold_right sepcon emp (map (atomic_entry sh) entries);
         entry_hists entries h)
   POST [ tvoid ]
-   EX i : Z, EX h' : list (hist * hist),
-   PROP (set_item_trace h key value i h')
+   EX i0 : Z, EX i : Z, EX h' : list (hist * hist),
+   PROP (set_item_trace h key value i0 i h')
    LOCAL ()
-   SEP (data_at sh (tarray (tptr tentry) 20) entries p;
+   SEP (data_at sh (tarray (tptr tentry) 32) entries p;
         fold_right sepcon emp (map (atomic_entry sh) entries);
         entry_hists entries h').
 (* set_item_trace_map describes the properties on the resulting map. *)
@@ -621,15 +683,16 @@ Definition failed_load k (a b : hist * hist) := exists t r, newer (fst a) t /\
    Conceptually, this is still linearizable because we could have just checked before the key was added,
    but at a finer-grained level we can tell the difference from the history, so we might as well keep
    this information. *)
-Definition get_item_trace (h : list (hist * hist)) k v i h' := 0 <= i < Zlength h /\
-  Forall2 (failed_load k) (sublist 0 i h) (sublist 0 i h') /\
+Definition get_item_trace (h : list (hist * hist)) k v i0 i h' := Zlength h' = Zlength h /\
+  0 <= i < Zlength h /\
   (let '(hk, hv) := Znth i h ([], []) in exists t r, newer hk t /\
      fst (Znth i h' ([], [])) = hk ++ [(t, Load (vint r))] /\
      (v = 0 /\ r = 0 /\ snd (Znth i h' ([], [])) = hv \/
       r = k /\ exists tv, Forall (fun x => fst x < tv)%nat hv /\
         snd (Znth i h' ([], [])) = hv ++ [(tv, Load (vint v))]) /\
     (let v := value_of_hist hk in v <> vint 0 -> v = vint r)) /\
-  sublist (i + 1) (Zlength h) h = sublist (i + 1) (Zlength h') h'.
+  forall j, (In j (indices i0 i) -> failed_load k (Znth j h ([], [])) (Znth j h' ([], []))) /\
+    (~In j (indices i0 i) -> j <> i -> Znth j h' ([], []) = Znth j h ([], [])).
 
 Lemma Znth_make_map : forall d h i (Hi : 0 <= i < Zlength h)
   (Hnz : Forall (fun x => value_of_hist (fst x) <> vint 0) (sublist 0 (i + 1) h))
@@ -907,16 +970,16 @@ Definition get_item_spec :=
  DECLARE _get_item
   WITH key : Z, p : val, sh : share, entries : list val, h : list (hist * hist), l : Z
   PRE [ _key OF tint, _value OF tint ]
-   PROP (repable_signed key; readable_share sh; key <> 0; Forall isptr entries; Zlength h = 20; wf_hists h l)
+   PROP (repable_signed key; readable_share sh; key <> 0; Forall isptr entries; Zlength h = 32; wf_hists h l)
    LOCAL (temp _key (vint key); gvar _m_entries p)
-   SEP (data_at sh (tarray (tptr tentry) 20) entries p;
+   SEP (data_at sh (tarray (tptr tentry) 32) entries p;
         fold_right sepcon emp (map (atomic_entry sh) entries);
         entry_hists entries h)
   POST [ tint ]
    EX value : Z, EX i : Z, EX h' : list (hist * hist),
    PROP (repable_signed value; get_item_trace h key value i h')
    LOCAL (temp ret_temp (vint value))
-   SEP (data_at sh (tarray (tptr tentry) 20) entries p;
+   SEP (data_at sh (tarray (tptr tentry) 32) entries p;
         fold_right sepcon emp (map (atomic_entry sh) entries);
         entry_hists entries h').
 
@@ -982,17 +1045,31 @@ Proof.
   forward_call key.
   Intro i'.
   eapply semax_pre with (P' := EX i : Z, EX i1 : Z, EX h' : list (hist * hist),
-    PROP (i1 mod 32 = (i' + i) mod 32; Forall2 (failed_CAS key) (sublist 0 i h) (sublist 0 i h');
-          sublist i (Zlength h) h = sublist i (Zlength h') h')
+    PROP (i1 mod 32 = (i' + i) mod 32; 0 <= i < 32;
+          forall j, if in_dec Z_eq_dec j (map (fun x => (i' + x) mod 32) (upto (Z.to_nat i)))
+            then failed_CAS key (Znth j h ([], [])) (Znth j h' ([], []))
+            else Znth j h' ([], []) = Znth j h ([], []))
     LOCAL (temp _idx (vint i1); temp _key (vint key); temp _value (vint value); gvar _m_entries p)
-    SEP (data_at sh (tarray (tptr tentry) 20) entries p; fold_right sepcon emp (map (atomic_entry sh) entries);
+    SEP (data_at sh (tarray (tptr tentry) 32) entries p; fold_right sepcon emp (map (atomic_entry sh) entries);
          entry_hists entries h')).
-  { Exists 0 i' h; rewrite sublist_nil; entailer!. }
+  { Exists 0 i' h; entailer!. }
   eapply semax_loop.
   - Intros i i1 h'; forward.
     forward.
+    rewrite sub_repr, and_repr; simpl.
+    rewrite Zland_two_p with (n := 5) by omega.
+    change (2 ^ 5) with 32.
+    exploit (Z_mod_lt i1 32); [omega | intro Hi1].
+    assert_PROP (Zlength entries = 32) as Hentries by entailer!.
+    rewrite <- Hentries in Hi1 at 3.
+    assert (isptr (Znth (i1 mod 32) entries Vundef)).
+    { apply Forall_Znth; auto. }
+    forward.
+    forward.
     assert (Zlength h' = Zlength h) as Hlen.
-    { assert (Zlength (sublist i (Zlength h) h) = Zlength (sublist i (Zlength h') h')) as Heq
+    { 
+
+assert (Zlength (sublist i (Zlength h) h) = Zlength (sublist i (Zlength h') h')) as Heq
         by (replace (sublist i (Zlength h) h) with (sublist i (Zlength h') h'); auto).
       rewrite !Zlength_sublist in Heq; try omega.
       destruct (Z_le_dec i (Zlength h')); [omega|].
@@ -1007,13 +1084,10 @@ Proof.
       rewrite sublist_split with (al := h)(mid := i) by omega.
       rewrite Hlen in *; rewrite !map_app; f_equal; [|congruence].
       eapply failed_CAS_fst; eauto. }
-    assert_PROP (Zlength entries = 20) by entailer!.
-    assert (0 <= i < Zlength entries) by (replace (Zlength entries) with 20; auto).
-    forward.
-    { entailer!.
-      apply isptr_is_pointer_or_null, Forall_Znth; auto. }
-    rewrite extract_nth_sepcon with (i := i), Znth_map with (d' := Vundef); try rewrite Zlength_map; auto.
-    unfold entry_hists; erewrite extract_nth_sepcon with (i := i)(l := map _ _), Znth_map, Znth_upto; simpl;
+    rewrite extract_nth_sepcon with (i := i1 mod 32), Znth_map with (d' := Vundef); try rewrite Zlength_map;
+      auto.
+Print entry_hists.
+    unfold entry_hists; erewrite extract_nth_sepcon with (i := i1)(l := map _ _), Znth_map, Znth_upto; simpl;
       auto; try omega.
     unfold atomic_entry; Intros lkey lval.
     rewrite atomic_loc_isptr.
